grammatik/Grammatik.lean
@@ -316,3 +316,5 @@ import Grammatik.ZeichenfolgeGebunden
 import Grammatik.Speichermodell.Sicht
 import Grammatik.Speichermodell.MaschineW
 import Grammatik.Speichermodell.DRF
+import Grammatik.Zielsatz.Schwach
+import Grammatik.Speichermodell.Zeuge
